kremlib/Spec.Loops.fst
@@ -30,51 +30,45 @@ let rec seq_map2 #a #b #c f s s' =
     let s'' = Seq.cons (f (Seq.head s) (Seq.head s')) (seq_map2 f (Seq.tail s) (Seq.tail s')) in
     s''
 
-val repeat_spec: #a:Type -> n:nat -> (f: a -> Tot a) -> a -> Tot a (decreases n)
-let rec repeat_spec #a n f x = if n = 0 then x else repeat_spec (n-1) f (f x)
+val repeat: #a:Type -> n:nat -> (f: a -> Tot a) -> a -> Tot a (decreases n)
+let rec repeat #a n f x =
+  if n = 0 then x else repeat (n-1) f (f x)
 
 #reset-options "--initial_fuel 2 --max_fuel 2"
 
-val lemma_repeat: #a:Type -> n:nat{n > 0} -> f:( a -> Tot a) -> x:a -> Lemma
-  (repeat_spec n f x == f (repeat_spec (n-1) f x))
-let rec lemma_repeat #a n f x =
+val repeat_induction: #a:Type -> n:nat{n > 0} -> f:( a -> Tot a) -> x:a -> Lemma
+  (repeat n f x == f (repeat (n-1) f x))
+let rec repeat_induction #a n f x =
   if n = 1 then ()
-  else lemma_repeat (n-1) f (f x)
+  else repeat_induction (n-1) f (f x)
 
-val lemma_repeat_0: #a:Type -> n:nat{n = 0} -> f:( a -> Tot a) -> x:a -> Lemma
-  (repeat_spec n f x == x)
-let rec lemma_repeat_0 #a n f x = ()
+val repeat_base: #a:Type -> n:nat{n = 0} -> f:( a -> Tot a) -> x:a -> Lemma
+  (repeat n f x == x)
+let rec repeat_base #a n f x = ()
 
 #reset-options "--max_fuel 0"
 
-val repeat_range_spec: #a:Type -> min:nat -> max:nat{min <= max} -> f:(a -> i:nat{i < max} -> Tot a) ->
+val repeat_range: #a:Type -> min:nat -> max:nat{min <= max} -> f:(a -> i:nat{i < max} -> Tot a) ->
   x:a -> Tot a (decreases (max - min))
-let rec repeat_range_spec #a min max f x =
+let rec repeat_range #a min max f x =
   if min = max then x
-  else repeat_range_spec (min+1) max f (f x min)
+  else repeat_range (min+1) max f (f x min)
 
 #reset-options "--initial_fuel 1 --max_fuel 1"
 
-val lemma_repeat_range_0: #a:Type -> min:nat -> max:nat{min <= max} -> f:(a -> i:nat{i < max} -> Tot a) -> x:a ->
-  Lemma (requires (min = max))
-        (ensures (repeat_range_spec min max f x == x))
-let lemma_repeat_range_0 #a min max f x = ()
-
-// JP: this lemma seems unused
-val lemma_repeat_range_1: #a:Type -> min:nat -> max:nat{min <= max} -> f:(a -> i:nat{i < max} -> Tot a) -> x:a ->
-  Lemma (requires (min <> max))
-        (ensures (min <> max /\ repeat_range_spec (min+1) max f (f x min) == repeat_range_spec min max f x))
-let lemma_repeat_range_1 #a min max f x = ()
+val repeat_range_base: #a:Type -> min:nat -> f:(a -> i:nat{i < min} -> Tot a) -> x:a ->
+  Lemma (ensures (repeat_range min min f x == x))
+let repeat_range_base #a min f x = ()
 
 #reset-options "--initial_fuel 2 --max_fuel 2"
 
-val lemma_repeat_range_spec:
+val repeat_range_induction:
   #a:Type -> min:nat -> max:nat{min < max} -> f:(a -> i:nat{i < max} -> Tot a) -> x:a -> 
   Lemma (requires (True))
-        (ensures f (repeat_range_spec min (max-1) f x) (max-1) == repeat_range_spec min max f x)
+        (ensures f (repeat_range min (max-1) f x) (max-1) == repeat_range min max f x)
         (decreases (max - min))
-let rec lemma_repeat_range_spec #a min max f x =
+let rec repeat_range_induction #a min max f x =
   if min = max - 1 then ()
-  else lemma_repeat_range_spec (min+1) max f (f x min)
+  else repeat_range_induction (min+1) max f (f x min)
 
 #reset-options "--max_fuel 0"
